Changed the mutual induction principle in typings.ott.
Using "Induction" instead of "Minimality" in Scheme for inductive
Prop's makes the induction principle weird, because the generated
principle can be used to prove things about propositions that depend
on the wf_* predicate itself. That leads to us proving statements of
the form

    Definition wf_something_prop
        a b c (H : wf_something a b c) := ...

    Theorem t : (forall a b c H, wf_something_prop a b c H) /\
        ...

instead of the more natural

    Definition wf_something_prop
        a b c := wf_something a b c ->

    Theorem t : (forall a b c, wf_something_prop a b c) /\
        ...

While trying to remove mutual induction from the development, it was
really hard to rewrite the theorems that had this form. Hopefully this
should make the task a tad easier now.



git-svn-id: https://webdav.seas.upenn.edu/svn/sol/vol@3871 eef5ea85-cc2e-0410-bd84-0fae1f012da8

src3.0/Transforms/memory_props.v
@@ -1617,8 +1617,8 @@ Proof.
          apply uninits_valid_ptrs.
 Qed.
 
-Definition zeroconst2GV_aux_disjoint_with_runtime_ptr_prop S td (t:typ) 
-  (H:wf_styp S td t) :=
+Definition zeroconst2GV_aux_disjoint_with_runtime_ptr_prop S td (t:typ) :=
+  wf_styp S td t ->
   forall los nts acc (Heq: td = (los, nts)) nts' 
   (Hsub:exists nts0, nts'=nts0++nts) (Huniq: uniq nts')
   maxb gl g mb ofs m
@@ -1631,8 +1631,8 @@ Definition zeroconst2GV_aux_disjoint_with_runtime_ptr_prop S td (t:typ)
           no_alias gv5 [(Vptr mb ofs, m)] /\ valid_ptrs (maxb + 1) gv5),
   no_alias g [(Vptr mb ofs, m)] /\ valid_ptrs (maxb + 1) g.
 
-Definition zeroconsts2GV_aux_disjoint_with_runtime_ptr_prop sdt 
-  (H:wf_styp_list sdt) :=
+Definition zeroconsts2GV_aux_disjoint_with_runtime_ptr_prop sdt :=
+  wf_styp_list sdt ->
   let 'lsdt := unmake_list_system_targetdata_typ sdt in
   let '(lsd, lt) := split lsdt in
   forall S td los nts acc (Heq: td = (los, nts)) nts' 
@@ -1648,8 +1648,8 @@ Definition zeroconsts2GV_aux_disjoint_with_runtime_ptr_prop sdt
   no_alias g [(Vptr mb ofs, m)] /\ valid_ptrs (maxb + 1) g.
 
 Lemma zeroconst2GV_aux_disjoint_with_runtime_ptr_mutrec :
-  (forall S TD t H, zeroconst2GV_aux_disjoint_with_runtime_ptr_prop S TD t H) /\
-  (forall sdt H, zeroconsts2GV_aux_disjoint_with_runtime_ptr_prop sdt H).
+  (forall S TD t, zeroconst2GV_aux_disjoint_with_runtime_ptr_prop S TD t) /\
+  (forall sdt, zeroconsts2GV_aux_disjoint_with_runtime_ptr_prop sdt).
 Proof.
   (wfstyp_cases (apply wf_styp_mutind; 
     unfold zeroconst2GV_aux_disjoint_with_runtime_ptr_prop, 
@@ -1676,14 +1676,14 @@ Case "wf_styp_structure".
     eapply wf_styp__feasible_typ_aux_mutrec_struct; eauto.
   subst. 
   inv_mbind. symmetry_ctx.
-  eapply H in HeqR0; eauto 2.
-  destruct g0; inv H1; auto.
+  eapply H1 in HeqR0; eauto 2.
+  destruct g0; inv H3; auto.
 
 Case "wf_styp_array".
   destruct sz5 as [|s]; 
     try solve [inv Hc2g; auto using uninits_valid_ptrs__disjoint_with_ptr].
     inv_mbind'. symmetry_ctx.
-    eapply H with (ofs:=ofs)(m:=m) in HeqR; eauto.
+    eapply H0 with (ofs:=ofs)(m:=m) in HeqR; eauto.
     assert (no_alias
       (g0 ++ uninits (Size.to_nat s0 - sizeGenericValue g0))
       [(Vptr mb ofs, m)] /\
@@ -1722,10 +1722,10 @@ Local Opaque no_alias valid_ptrs.
   destruct R as [lsd lt]. simpl.
   intros. subst. 
   apply eq_system_targetdata_cons_inv in Heq'. 
-  destruct Heq' as [H2 [EQ1 EQ2]]; subst. uniq_result.
+  destruct Heq' as [H4 [EQ1 EQ2]]; subst. uniq_result.
   inv_mbind. symmetry_ctx.
-  eapply H in HeqR1; eauto 1. clear H.
-  eapply H0 in HeqR0; eauto 1. clear H0.
+  eapply H0 in HeqR1; eauto 1. clear H0.
+  eapply H2 in HeqR0; eauto 1. clear H2.
   destruct HeqR1. destruct HeqR0.
   split.
     apply no_alias_app; auto.
@@ -1841,16 +1841,16 @@ Proof.
     assert (H1:=@H b i0). congruence.
 Qed.
 
-Definition const2GV_disjoint_with_runtime_ptr_prop S td c t 
-  (H:wf_const S td c t) :=
+Definition const2GV_disjoint_with_runtime_ptr_prop S td c t :=
+  wf_const S td c t ->
   forall maxb gl g mb t0 ofs m
   (Hwfg: wf_globals maxb gl)
   (Hc2g : _const2GV td gl c = ret (g, t0))
   (Hle: maxb < mb),
   t = t0 /\ no_alias g [(Vptr mb ofs, m)] /\ valid_ptrs (maxb+1) g.
 
-Definition list_const2GV_disjoint_with_runtime_ptr_prop sdct 
-  (H:wf_const_list sdct) :=
+Definition list_const2GV_disjoint_with_runtime_ptr_prop sdct :=
+  wf_const_list sdct ->
   let 'lsdct := unmake_list_system_targetdata_const_typ sdct in
   let '(lsdc, lt) := split lsdct in
   let '(lsd, lc) := split lsdc in
@@ -1871,8 +1871,8 @@ Definition list_const2GV_disjoint_with_runtime_ptr_prop sdct
   ).
 
 Lemma const2GV_disjoint_with_runtime_ptr_mutrec :
-  (forall S td c t H, const2GV_disjoint_with_runtime_ptr_prop S td c t H) /\
-  (forall sdct H, list_const2GV_disjoint_with_runtime_ptr_prop sdct H).
+  (forall S td c t, const2GV_disjoint_with_runtime_ptr_prop S td c t) /\
+  (forall sdct, list_const2GV_disjoint_with_runtime_ptr_prop sdct).
 Proof.
   (wfconst_cases (apply wf_const_mutind; 
                   unfold const2GV_disjoint_with_runtime_ptr_prop, 
@@ -1911,19 +1911,19 @@ Case "wfconst_array". Focus.
         | 0%nat => _
         | S _ => _ 
         end = _ |- _ => 
-  rewrite e in H3; unfold Size.to_nat in *;
+  rewrite H1 in H3; unfold Size.to_nat in *;
   destruct sz5; inv H3; split; auto
   end.
     simpl. auto.
 
-    destruct (@H system5 targetdata5 maxb gl mb ofs m) as [J1 J2]; 
+    destruct (@H0 system5 targetdata5 maxb gl mb ofs m) as [J1 J2]; 
       try solve 
       [destruct targetdata5; eauto using const2GV_typsize_mutind_array'].
     symmetry_ctx.
     assert (make_list_const lc = const_list) as EQ.
       eapply make_list_const_spec2; eauto.
     rewrite <- EQ in HeqR. subst.
-    rewrite length_unmake_make_list_const in e. 
+    rewrite length_unmake_make_list_const in H1. 
     apply J1 in HeqR; eauto using make_list_const_spec4.
 Unfocus.
 
@@ -1940,15 +1940,15 @@ Case "wfconst_struct". Focus.
   destruct R' as [lsd lc].
   remember (split lsd) as R''.
   destruct R'' as [ls ld].
-  destruct (@H system5 (layouts5, namedts5) maxb gl mb ofs m) as [J1 J2];
+  destruct (@H0 system5 (layouts5, namedts5) maxb gl mb ofs m) as [J1 J2];
     eauto using const2GV_typsize_mutind_struct'.
   destruct_if.
-  destruct g0; inv H2.
+  destruct g0; inv H5.
     split; simpl; auto.
     split; auto.
       symmetry in HeqR.
       erewrite <- map_list_const_typ_spec2 in HeqR; eauto.
-      erewrite <- map_list_const_typ_spec1 in e; eauto.
+      erewrite <- map_list_const_typ_spec1 in H2; eauto.
       apply J2 in HeqR.
       destruct HeqR as [J5 [J6 J7]]; subst.
       split; eauto using uninits_valid_ptrs__disjoint_with_ptr.
@@ -1994,7 +1994,7 @@ Case "wfconst_inttoptr".
     eauto using undef_valid_ptrs.
 Case "wfconst_bitcast".
   symmetry_ctx.
-  eapply H in HeqR; eauto. destruct HeqR as [J1 [J2 J3]].
+  eapply H0 in HeqR; eauto. destruct HeqR as [J1 [J2 J3]].
   assert (mcast targetdata5 castop_bitcast t (typ_pointer typ2) g0 = ret g) 
     as J.
     simpl. auto.
@@ -2004,16 +2004,16 @@ Case "wfconst_bitcast".
     eapply mcast_preserves_valid_ptrs; eauto.
 Case "wfconst_gep". Focus.
   symmetry in HeqR.
-  eapply H with (ofs:=ofs)(m:=m) in HeqR; eauto.
+  eapply H0 with (ofs:=ofs)(m:=m) in HeqR; eauto.
   destruct HeqR as [J1 [J2 J3]]; subst.
   remember (getConstGEPTyp const_list (typ_pointer typ5)) as R2.
-  destruct R2; tinv H2. uniq_result.
+  destruct R2; tinv H8. uniq_result.
   remember (GV2ptr targetdata5 (getPointerSize targetdata5) g0) as R3.
-  destruct R3; tinv H2.
+  destruct R3; tinv H8.
     remember (intConsts2Nats targetdata5 const_list) as R4.
-    destruct R4; tinv H2.
+    destruct R4; tinv H8.
       remember (mgep targetdata5 typ5 v l0) as R5.
-      destruct R5; inv H2.
+      destruct R5; inv H8.
         symmetry_ctx. uniq_result. 
         split; auto.
         split.
@@ -2037,16 +2037,16 @@ Case "wfconst_icmp".
     eapply micmp_preserves_no_alias; eauto.
     eapply micmp_preserves_valid_ptrs; eauto.
 Case "wfconst_fcmp".
-  destruct t; tinv H2. inv_mbind'.
+  destruct t; tinv H8. inv_mbind'.
   split; auto.
   split.
     eapply mfcmp_preserves_no_alias; eauto.
     eapply mfcmp_preserves_valid_ptrs; eauto.
 Case "wfconst_extractvalue".
   symmetry_ctx.
-  eapply H in HeqR; eauto.
+  eapply H0 in HeqR; eauto.
   destruct HeqR as [J1 [J2 J3]]; subst.
-  destruct e0 as [idxs [o [J5 J4]]].
+  destruct H6 as [idxs [o [J5 J4]]].
   eapply getSubTypFromConstIdxs__mgetoffset in HeqR0; eauto.
   subst.
   split; auto.
@@ -2055,8 +2055,8 @@ Case "wfconst_extractvalue".
     eapply extractGenericValue_preserves_valid_ptrs; eauto.
 Case "wfconst_insertvalue".
   symmetry_ctx.
-  eapply H in HeqR; eauto. clear H.
-  eapply H0 in HeqR0; eauto. clear H0 H1.
+  eapply H0 in HeqR; eauto. clear H0.
+  eapply H2 in HeqR0; eauto. clear H2 H3.
   destruct HeqR as [J1 [J2 J3]]; subst.
   destruct HeqR0 as [J4 [J5 J6]]; subst.
   split; auto.
@@ -2065,11 +2065,11 @@ Case "wfconst_insertvalue".
     eapply insertGenericValue_preserves_no_alias in HeqR1; eauto.
     eapply insertGenericValue_preserves_valid_ptrs in HeqR1; eauto.
 Case "wfconst_bop".
-  destruct t; tinv H2. inv_mbind'.
+  destruct t; tinv H5. inv_mbind'.
   symmetry_ctx. 
-  eapply H with (ofs:=ofs)(m:=m) in HeqR; eauto.
+  eapply H0 with (ofs:=ofs)(m:=m) in HeqR; eauto.
   destruct HeqR as [J1 [J2 J3]]; subst.
-  eapply H0 with (ofs:=ofs)(m:=m) in HeqR0; eauto.
+  eapply H2 with (ofs:=ofs)(m:=m) in HeqR0; eauto.
   destruct HeqR0 as [J4 [J5 J6]]; subst.
   uniq_result.
   split; auto.
@@ -2077,11 +2077,11 @@ Case "wfconst_bop".
     eapply mbop_preserves_no_alias; eauto.
     eapply mbop_preserves_valid_ptrs; eauto.
 Case "wfconst_fbop".
-  destruct t; tinv H2. inv_mbind'.
+  destruct t; tinv H5. inv_mbind'.
   symmetry_ctx. 
-  eapply H with (ofs:=ofs)(m:=m) in HeqR; eauto.
+  eapply H0 with (ofs:=ofs)(m:=m) in HeqR; eauto.
   destruct HeqR as [J1 [J2 J3]]; subst.
-  eapply H0 with (ofs:=ofs)(m:=m) in HeqR0; eauto.
+  eapply H2 with (ofs:=ofs)(m:=m) in HeqR0; eauto.
   destruct HeqR0 as [J4 [J5 J6]]; subst.
   uniq_result.
   split; auto.
@@ -2107,14 +2107,14 @@ Local Opaque no_alias.
   remember (split lsd) as R3.
   destruct R3 as [ls ld].
   split; intros; simpl in *; inv_mbind'.
-    destruct (typ_dec t t0); tinv H3.
+    destruct (typ_dec t t0); tinv H5.
     inv_mbind'. symmetry_ctx.
     apply wf_list_targetdata_typ_cons_inv' in Hwfls.
     destruct Hwfls as [J1 [J2 J3]]; subst.
-    eapply H with (ofs:=ofs)(m:=m) in HeqR0; eauto.
+    eapply H0 with (ofs:=ofs)(m:=m) in HeqR0; eauto.
     destruct HeqR0 as [J5 [J6 J7]]; subst.
-    eapply H0 with (ofs:=ofs)(m:=m) in HeqR; eauto. 
-    destruct HeqR as [J8 J9]. clear H H0.
+    eapply H2 with (ofs:=ofs)(m:=m) in HeqR; eauto. 
+    destruct HeqR as [J8 J9]. clear H0 H2.
     split.
       apply no_alias_app; auto.
         apply no_alias_app; auto.
@@ -2126,10 +2126,10 @@ Local Opaque no_alias.
     apply wf_list_targetdata_typ_cons_inv' in Hwfls.
     destruct Hwfls as [J1' [J2' J3]]; subst.
     symmetry_ctx.
-    eapply H with (ofs:=ofs)(m:=m) in HeqR0; eauto.
+    eapply H0 with (ofs:=ofs)(m:=m) in HeqR0; eauto.
     destruct HeqR0 as [J5 [J6 J7]]; subst.
-    eapply H0 with (ofs:=ofs)(m:=m) in HeqR; eauto. 
-    destruct HeqR as [J8 [J9 J10]]; subst. clear H H0.
+    eapply H2 with (ofs:=ofs)(m:=m) in HeqR; eauto. 
+    destruct HeqR as [J8 [J9 J10]]; subst. clear H0 H2.
     split; auto.
     split.
       apply no_alias_app; auto.
